A much improved version of the interpretation combinator

ITree_Interp.thy
@@ -2,14 +2,146 @@ theory ITree_Interp
   imports ITrees "Optics.Optics"
 begin
 
+definition pfun_singleton :: "('a \<Zpfun> 'b) \<Rightarrow> bool" where
+"pfun_singleton f = (\<exists> k v. f = {k \<mapsto> v}\<^sub>p)" 
+
+lemma pfun_singleton_maplet [simp]:
+  "pfun_singleton {k \<mapsto> v}\<^sub>p"
+  by (auto simp add: pfun_singleton_def)
+
+definition dest_pfsingle :: "('a \<Zpfun> 'b) \<Rightarrow> 'a \<times> 'b" where
+"dest_pfsingle f = (THE (k, v). f = {k \<mapsto> v}\<^sub>p)"
+
+lemma dest_pfsingle_maplet [simp]: "dest_pfsingle {k \<mapsto> v} = (k, v)"
+  apply (auto intro!:the_equality simp add: dest_pfsingle_def)
+  apply (metis pdom_upd pdom_zero singleton_insert_inj_eq)
+  apply (metis pdom_upd pdom_zero pfun_app_upd_1 singleton_insert_inj_eq)
+  done  
+
+definition RPC :: "('a \<Longrightarrow>\<^sub>\<triangle> 'e) \<Rightarrow> 'a \<Rightarrow> ('b \<Longrightarrow>\<^sub>\<triangle> 'e) \<Rightarrow> ('b \<Rightarrow> ('e, 'r) itree) \<Rightarrow> ('e, 'r) itree" where
+"RPC a v b P = Vis {build\<^bsub>a\<^esub> v \<mapsto> Vis {b x \<Rightarrow> P x}\<^sub>p}" 
+
+lemma is_Vis_RPC [simp]: "is_Vis (RPC a v b P)"
+  by (simp add: RPC_def)
+
+lemma RPC_val_eq: "wb_prism a \<Longrightarrow> RPC a v1 b P1 = RPC a v2 b P2 \<Longrightarrow> v1 = v2"
+  by (metis RPC_def dest_pfsingle_maplet itree.simps(3) option.simps(1) prod.simps(1) wb_prism.match_build)
+
+lemma RPC_cont_eq: "wb_prism b \<Longrightarrow> RPC a v b P1 = RPC a v b P2 \<Longrightarrow> P1 = P2"
+  by (simp add: RPC_def pfun_eq_iff prism_fun_def prism_fun_upd_def fun_eq_iff)
+
+definition is_RPC :: "('a \<Longrightarrow>\<^sub>\<triangle> 'e) \<Rightarrow> ('b \<Longrightarrow>\<^sub>\<triangle> 'e) \<Rightarrow> ('e, 'r) itree \<Rightarrow> bool" where
+"is_RPC a b P = (case P of
+                   Vis F \<Rightarrow> (if pfun_singleton F
+                             then (let (e, P') = dest_pfsingle F 
+                                   in if e \<in> range build\<^bsub>a\<^esub>
+                                      then case F e of 
+                                             Vis F' \<Rightarrow> dom F' = range build\<^bsub>b\<^esub> | 
+                                             _ \<Rightarrow> False
+                                      else False)
+                             else False) | 
+                   _ \<Rightarrow> False)"
+
+lemma is_RPC_RPC [simp]: "is_RPC a b (RPC a v b P)"
+  by (auto simp add: RPC_def is_RPC_def prism_fun_def prism_fun_upd_def)
+
+definition dest_RPC :: "('a \<Longrightarrow>\<^sub>\<triangle> 'e) \<Rightarrow> ('b \<Longrightarrow>\<^sub>\<triangle> 'e) \<Rightarrow> ('e, 'r) itree \<Rightarrow> ('a \<times> ('b \<Rightarrow> ('e, 'r) itree))" where
+"dest_RPC a b P = (let F = un_Vis P; 
+                      (e, P') = dest_pfsingle F;  
+                      F' = un_Vis P' 
+                      in (the (match\<^bsub>a\<^esub> e), \<lambda> v. F' (build\<^bsub>b\<^esub> v)))"
+
+lemma dest_RPC_RPC [simp]: "\<lbrakk> wb_prism a; wb_prism b \<rbrakk> \<Longrightarrow> dest_RPC a b (RPC a v b P) = (v, P)"
+  by (simp add: dest_RPC_def RPC_def)
+  
 definition iter :: "('a \<Rightarrow> ('e, 'a + 'b) itree) \<Rightarrow> 'a \<Rightarrow> ('e, 'b) itree"
-  where "iter P s = iterate (\<lambda> s. \<not> isl s) (P \<circ> projl) (Inl s) \<bind> Ret \<circ> projr"
+  where "iter P s = iterate isl (P \<circ> projl) (Inl s) \<bind> Ret \<circ> projr"
+
+(* The funny redness happens when you try to make a monomorphic friend function polymorphic *)
+
+(*
+corec interp :: "'e set \<Rightarrow> ('e \<Rightarrow> ('e, 'r) itree) \<Rightarrow> ('e, 'r) itree \<Rightarrow> ('e, 'r) itree" where
+"interp E P Q =
+  (case Q of 
+    Ret x  \<Rightarrow> Ret x 
+  | Sil Q' \<Rightarrow> Sil (interp E P Q')
+  | Vis F  \<Rightarrow> if pfun_singleton F \<and> dom F \<subseteq> E
+              then let (e, Q') = dest_pfsingle F
+                   in P e \<bind> (\<lambda> _. Sil (interp E P Q'))
+              else Vis (map_pfun (interp E P) F))"
+*)
+
+corec interp :: "('a \<Longrightarrow>\<^sub>\<triangle> 'e) \<Rightarrow> ('r \<Longrightarrow>\<^sub>\<triangle> 'e) \<Rightarrow> ('a \<Rightarrow> ('e, 'r) itree) \<Rightarrow> ('e, 'r) itree \<Rightarrow> ('e, 'r) itree" where
+"interp a b P Q = 
+  (case Q of 
+    Ret x  \<Rightarrow> Ret x 
+  | Sil Q' \<Rightarrow> Sil (interp a b P Q') 
+  | Vis F  \<Rightarrow> if is_RPC a b (Vis F)
+              then let (v, Q') = dest_RPC a b (Vis F)
+                   in \<tau> (interp a b P (P v)) \<bind> (\<lambda> x. \<tau> (interp a b P (Q' x)))
+              else Vis (map_pfun (interp a b P) F))"
+
+lemma case_itree_RPC: "case_itree R S V (RPC a v b P) = (V (un_Vis (RPC a v b P)))"
+  by (simp add: RPC_def)
+
+chantype ch =
+  a :: int
+  ar :: int
+
+lemma "interp a ar (\<lambda> n. Ret (n + 1)) (RPC a 5 ar Ret) = \<tau> (\<tau> (\<checkmark> 6))"
+  apply (subst interp.code)
+  apply (simp add: case_itree_RPC)
+  apply (subst interp.code)
+  apply (simp add: case_itree_RPC)
+  apply (subst interp.code)
+  apply (simp add: case_itree_RPC)
+  done
+
+chantype ch2 =
+  cnt :: int
+  b :: int
+  br :: unit
+
+definition pfx :: "'e \<Rightarrow> ('e, 's) itree \<Rightarrow>('e, 's) itree" where
+"pfx e P = Vis {e \<mapsto> P}"
+
+
+lemma "interp b br (\<lambda> n. pfx (build\<^bsub>cnt\<^esub> n) (RPC b (n + 1) br (\<lambda> _. Ret ()))) (RPC b 0 br (\<lambda> _. Ret ())) = undefined"
+  apply (subst interp.code)
+  apply (simp add: case_itree_RPC)
+  apply (subst interp.code)
+  apply (simp add: case_itree_RPC pfx_def)
+  oops
+
+(*
+definition interp :: "('a \<Longrightarrow>\<^sub>\<triangle> 'e) \<Rightarrow> ('b \<Longrightarrow>\<^sub>\<triangle> 'e) \<Rightarrow> ('a \<Rightarrow> ('e, 'b) itree) \<Rightarrow> ('e, 'r) itree \<Rightarrow> ('e, 'r) itree" where
+"interp c d I P = 
+  iter (\<lambda> Q::('e, 'r) itree. 
+    (case Q of 
+      Sil Q' \<Rightarrow> Ret (Inl Q') |
+      Ret x \<Rightarrow> Ret (Inr x) |
+      Vis F \<Rightarrow> if pfun_singleton F
+               then (let (e, P') = dest_pfsingle F in 
+                     case P' of 
+                       Vis F' \<Rightarrow> )
+               else diverge)) P"
+*)
+
+(*
+map_itree ((\<lambda> a. if (build\<^bsub>c\<^esub> a \<in> pdom(F))
+                           then Inl (F (build\<^bsub>c\<^esub>a)\<^sub>p) 
+                           else Inl deadlock) :: 'a \<Rightarrow> ('e, 'r) itree + 'r) I
+    )) P"
+*)
+
 
 text \<open> Here, I is effectively pushing the buttons of P, by providing the events that P needs
-  to continue. \<close>
+  to continue. The loop (@{const iter}) steps through each constructor of @{term P}, returning
+  the successor ITree at each step, or terminating if a return is encountered. If a visible event
+  is encountered, the ITree @{term I} is executed to provide an event input for @{term P}. \<close>
 
-definition interp :: "('a \<Longrightarrow>\<^sub>\<triangle> 'e) \<Rightarrow> ('e, 'a) itree \<Rightarrow> ('e, 'r) itree \<Rightarrow> ('e, 'r) itree" where
-"interp c I P = 
+definition interpO :: "('a \<Longrightarrow>\<^sub>\<triangle> 'e) \<Rightarrow> ('e, 'a) itree \<Rightarrow> ('e, 'r) itree \<Rightarrow> ('e, 'r) itree" where
+"interpO c I P = 
   iter (\<lambda> Q::('e, 'r) itree. 
     (case Q of 
       Sil Q' \<Rightarrow> Ret (Inl Q') |
